<?xml version="1.0"?>


<!DOCTYPE rdf:RDF [
    <!ENTITY owl "http://www.w3.org/2002/07/owl#" >
    <!ENTITY swrl "http://www.w3.org/2003/11/swrl#" >
    <!ENTITY owl2 "http://www.w3.org/2006/12/owl2#" >
    <!ENTITY xsd "http://www.w3.org/2001/XMLSchema#" >
    <!ENTITY rdfs "http://www.w3.org/2000/01/rdf-schema#" >
    <!ENTITY rdf "http://www.w3.org/1999/02/22-rdf-syntax-ns#" >
]>


<rdf:RDF xmlns="http://www.descartes-core.org/patterns/owl/transportPattern#"
     xml:base="http://www.descartes-core.org/patterns/owl/transportPattern"
     xmlns:rdfs="http://www.w3.org/2000/01/rdf-schema#"
     xmlns:swrl="http://www.w3.org/2003/11/swrl#"
     xmlns:owl="http://www.w3.org/2002/07/owl#"
     xmlns:xsd="http://www.w3.org/2001/XMLSchema#"
     xmlns:rdf="http://www.w3.org/1999/02/22-rdf-syntax-ns#"
     xmlns:owl2="http://www.w3.org/2006/12/owl2#"
     xmlns:cpannotationschema="http://www.ontologydesignpatterns.org/schemas/cpannotationschema.owl#">
    <owl:Ontology rdf:about="http://www.descartes-core.org/patterns/owl/transportPattern">
        <rdfs:label rdf:datatype="&rdf;PlainLiteral">Transport Pattern</rdfs:label>
        <owl:versionInfo rdf:datatype="&xsd;string">0.1</owl:versionInfo>
        <cpannotationschema:scenarios rdf:datatype="&xsd;string">The rive water has pollution from a location, after a certain time.  A package left Auckland, New Zealand, at 5:45am on 01/06/2012 and arrived in Los Angeles, USA, on 01/12/2012.</cpannotationschema:scenarios>
        <owl:versionInfo rdf:datatype="&xsd;string">Created by Brandon Whitehead</owl:versionInfo>
        <cpannotationschema:relatedCPs rdf:datatype="&xsd;string">No known CPs at this time.</cpannotationschema:relatedCPs>
        <cpannotationschema:hasConsequences rdf:datatype="&xsd;string">This CP allows data modellers and ontology creators the ability to filter and categorise large geoscience data stores.</cpannotationschema:hasConsequences>
        <cpannotationschema:hasIntent rdf:datatype="&xsd;string">To reduce dimensionality of large data collections.</cpannotationschema:hasIntent>
        <cpannotationschema:coversRequirements rdf:datatype="&xsd;string">What is the extent of a point source pollution event? Where did a voyage begin, and where did it end?</cpannotationschema:coversRequirements>
        <owl:imports rdf:resource="http://www.ontologydesignpatterns.org/schemas/cpannotationschema.owl"/>
    </owl:Ontology>
    


    <!-- 
    ///////////////////////////////////////////////////////////////////////////////////////
    //
    // Object Properties
    //
    ///////////////////////////////////////////////////////////////////////////////////////
     -->

    


    <!-- http://www.descartes-core.org/patterns/owl/transportPattern#partOf -->

    <owl:ObjectProperty rdf:about="http://www.descartes-core.org/patterns/owl/transportPattern#partOf">
        <rdf:type rdf:resource="&owl;TransitiveProperty"/>
        <rdfs:label xml:lang="en">part of</rdfs:label>
    </owl:ObjectProperty>
    
    <!-- http://www.descartes-core.org/patterns/owl/transportPattern#referenceFrame -->    
    
    <owl:ObjectProperty rdf:about="http://www.descartes-core.org/patterns/owl/transportPattern#referenceFrame">
        <rdfs:label xml:lang="en">reference frame</rdfs:label>
        <rdfs:domain rdf:resource="http://www.descartes-core.org/patterns/owl/transportPattern#transportEvent"/>
        <rdfs:range rdf:resource="http://www.descartes-core.org/patterns/owl/transportPattern#transportEvent"/>
        <rdfs:comment>This property is significant in that it serves to restrict and disambiguate a myriad of inherent facets, often in juxtaposition, associated with the Earths complex phenomena. The reference frame is provided to restrict the input values for a given instantiation, inherently providing context to the local representation.</rdfs:comment>
    </owl:ObjectProperty>
    


    <!-- 
    ///////////////////////////////////////////////////////////////////////////////////////
    //
    // Classes
    //
    ///////////////////////////////////////////////////////////////////////////////////////
     -->

    


    <!-- http://www.descartes-core.org/patterns/owl/transportPattern#TransportEntity -->

    <owl:Class rdf:about="http://www.descartes-core.org/patterns/owl/transportPattern#TransportEntity">
        <rdfs:subClassOf rdf:resource="&owl;Thing"/>
        <rdfs:subClassOf>
            <owl:Restriction>
                <owl:onProperty rdf:resource="http://www.descartes-core.org/patterns/owl/transportPattern#partOf"/>
                <owl:someValuesFrom rdf:resource="http://www.descartes-core.org/patterns/owl/transportPattern#TransportEvent"/>
            </owl:Restriction>
        </rdfs:subClassOf>
        <rdfs:label xml:lang="en">Transport Entity</rdfs:label>
        <rdfs:comment>The Transport Entity concept represents the identity of the circumscribed portion of energy or mass that is moved.</rdfs:comment>
    </owl:Class>
    


    <!-- http://www.descartes-core.org/patterns/owl/transportPattern#TransportEvent -->

    <owl:Class rdf:about="http://www.descartes-core.org/patterns/owl/transportPattern#TransportEvent">
        <rdfs:label xml:lang="en">Transport Event</rdfs:label>
        <rdfs:comment>A Transport Event describes a specific transport phenomenon, as movement of some mass or energy (measurable entity) from one location to another, based on a common and persistent frame of reference.</rdfs:comment>
    </owl:Class>
    


    <!-- http://www.descartes-core.org/patterns/owl/transportPattern#TransportMechanim -->

    <owl:Class rdf:about="http://www.descartes-core.org/patterns/owl/transportPattern#TransportMechanim">
        <rdfs:subClassOf rdf:resource="&owl;Thing"/>
        <rdfs:subClassOf>
            <owl:Restriction>
                <owl:onProperty rdf:resource="http://www.descartes-core.org/patterns/owl/transportPattern#partOf"/>
                <owl:someValuesFrom rdf:resource="http://www.descartes-core.org/patterns/owl/transportPattern#TransportEvent"/>
            </owl:Restriction>
        </rdfs:subClassOf>
        <rdfs:label xml:lang="en">Transport Mechanism</rdfs:label>
        <rdfs:comment>The transportMechanism concept captures the nature of the source that acts upon the transportEntity, and thus induces a transportEvent.</rdfs:comment>
    </owl:Class>
</rdf:RDF>



<!-- Generated by the OWL API (version 3.2.0.1502) http://owlapi.sourceforge.net -->

