@prefix : <https://patternKindOfXAndXOfInterest/> .
@prefix owl: <http://www.w3.org/2002/07/owl#> .
@prefix rdf: <http://www.w3.org/1999/02/22-rdf-syntax-ns#> .
@prefix xml: <http://www.w3.org/XML/1998/namespace> .
@prefix xsd: <http://www.w3.org/2001/XMLSchema#> .
@prefix rdfs: <http://www.w3.org/2000/01/rdf-schema#> .
@prefix skos: <http://www.w3.org/2004/02/skos/core#> .
@prefix untitled-ontology-238: <https://opendata.inrae.fr/untitled-ontology-238#> .
@base <https://patternKindOfXAndXOfInterest/> .

<https://patternKindOfXAndXOfInterest> rdf:type owl:Ontology ;
                                        owl:imports <http://www.w3.org/2004/02/skos/core> .

#################################################################
#    Object Properties
#################################################################

###  https://patternKindOfXAndXOfInterest#hasKind
:hasKind rdf:type owl:ObjectProperty ;
         skos:definition "The hasKind property binds a specific entity (instance of class XOfInterest) to its archetypes (instance of class XKind)."@en .


###  https://patternKindOfXAndXOfInterest#hasX
:hasX rdf:type owl:ObjectProperty ;
      owl:inverseOf :isXOf ;
      rdfs:range :X ;
      skos:definition "The hasX property binds any entity to an instance of class X."@en .


###  https://patternKindOfXAndXOfInterest#hasXKind
:hasXKind rdf:type owl:ObjectProperty ;
          rdfs:subPropertyOf :hasX ;
          owl:inverseOf :isXKindOf ;
          rdfs:range :XKind ;
          skos:definition "The hasXKind property binds any entity to an instance of class XKind."@en .


###  https://patternKindOfXAndXOfInterest#hasXOfInterest
:hasXOfInterest rdf:type owl:ObjectProperty ;
                rdfs:subPropertyOf :hasX ;
                owl:inverseOf :isXOfInterestOf ;
                rdfs:range :XOfInterest ;
                skos:definition "The hasXOfInterest property binds any entity to an instance of class XOfInterest."@en .


###  https://patternKindOfXAndXOfInterest#isXKindOf
:isXKindOf rdf:type owl:ObjectProperty ;
           rdfs:subPropertyOf :isXOf ;
           rdfs:domain :XKind ;
           skos:definition "The isXKindOf property binds an instance of class XKind to any entity."@en .


###  https://patternKindOfXAndXOfInterest#isXOf
:isXOf rdf:type owl:ObjectProperty ;
       rdfs:domain :X ;
       skos:definition "The isXOf property binds an instance of class X to any entity."@en .


###  https://patternKindOfXAndXOfInterest#isXOfInterestOf
:isXOfInterestOf rdf:type owl:ObjectProperty ;
                 rdfs:subPropertyOf :isXOf ;
                 rdfs:domain :XOfInterest ;
                 skos:definition "The isXOfInterestOf property binds an instance of class XOfInterest to any entity."@en .


#################################################################
#    Classes
#################################################################

###  https://patternKindOfXAndXOfInterest#X
:X rdf:type owl:Class ;
   skos:definition "The class X (e.g. Feature, Property, Device) represents the class of entities whose type is indeterminate (neither archetype nor specific). It can be specialized in a class hierarchy. The class X is equivalent to the disjoint union of XKind and XOfInterest"@en .


###  https://patternKindOfXAndXOfInterest#XKind
:XKind rdf:type owl:Class ;
       rdfs:subClassOf skos:Concept ,
                       :X ;
       skos:definition "The class XKind represent the class of archetypes of X. XKind is a subclass of skos:Concept, and these instances are organized into a SKOS model using the skos:broader and skos:narrower properties. Local restrictions on XKind force more specific and more generic concepts to also be of type XKind."@en .


###  https://patternKindOfXAndXOfInterest#XOfInterest
:XOfInterest rdf:type owl:Class ;
             rdfs:subClassOf :X ;
             skos:definition "The class XOfInterest represents specific X."@en .


###  Generated by the OWL API (version 4.5.25.2023-02-15T19:15:49Z) https://github.com/owlcs/owlapi
