<?xml version="1.0"?>
<rdf:RDF xmlns="https://w3id.org/smartenvironment/patterns/sensing.owl#"
     xml:base="https://w3id.org/smartenvironment/patterns/sensing.owl"
     xmlns:schema="http://schema.org/"
     xmlns:rdf="http://www.w3.org/1999/02/22-rdf-syntax-ns#"
     xmlns:terms="http://purl.org/dc/terms/"
     xmlns:owl="http://www.w3.org/2002/07/owl#"
     xmlns:xml="http://www.w3.org/XML/1998/namespace"
     xmlns:cpannotationschema="http://www.ontologydesignpatterns.org/schemas/cpannotationschema.owl#"
     xmlns:xsd="http://www.w3.org/2001/XMLSchema#"
     xmlns:skos="http://www.w3.org/2004/02/skos/core#"
     xmlns:rdfs="http://www.w3.org/2000/01/rdf-schema#"
     xmlns:se-sensing="https://w3id.org/smartenvironment/patterns/sensing.owl#"
     xmlns:vann="http://purl.org/vocab/vann/"
     xmlns:foaf="http://xmlns.com/foaf/0.1/">
    <owl:Ontology rdf:about="https://w3id.org/smartenvironment/patterns/sensing">
        <owl:imports rdf:resource="http://www.w3.org/ns/ssn/"/>
        <cpannotationschema:coversRequirements xml:lang="en">What sensors make a sensing (observation) process?</cpannotationschema:coversRequirements>
        <vann:preferredNamespacePrefix xml:lang="en">se-sensing</vann:preferredNamespacePrefix>
        <vann:preferredNamespaceUri rdf:resource="https://w3id.org/smartenvironment/patterns/sensing.owl"/>
        <terms:description xml:lang="en">This ontology mainly relies on the SSN ontology (http://www.w3.org/ns/ssn/) and describes a sensing process in the context on smart environment. It provides information about the sensors, the observation process and the configuration of the sensors.</terms:description>
        <rdfs:seeAlso rdf:resource="http://www.w3.org/ns/ssn/"/>
        <cpannotationschema:coversRequirements xml:lang="en">What are the feature of interests considered within an observation proces?</cpannotationschema:coversRequirements>
        <cpannotationschema:isSpecializationOf rdf:resource="http://www.w3.org/ns/ssn/"/>
        <terms:created xml:lang="en">2017-10-22</terms:created>
        <cpannotationschema:coversRequirements xml:lang="en">What is the output (result) of a sensing process?</cpannotationschema:coversRequirements>
        <terms:title xml:lang="en">Smart Environment Sensing Ontology Pattern</terms:title>
    </owl:Ontology>
    


    <!-- 
    ///////////////////////////////////////////////////////////////////////////////////////
    //
    // Classes
    //
    ///////////////////////////////////////////////////////////////////////////////////////
     -->

    


    <!-- https://w3id.org/smartenvironment/patterns/sensing.owl#ConfigurationProcedure -->

    <owl:Class rdf:about="https://w3id.org/smartenvironment/patterns/sensing.owl#ConfigurationProcedure">
        <rdfs:subClassOf rdf:resource="http://www.w3.org/ns/sosa/Procedure"/>
        <rdfs:subClassOf>
            <owl:Restriction>
                <owl:onProperty rdf:resource="http://www.w3.org/ns/ssn/implementedBy"/>
                <owl:someValuesFrom rdf:resource="https://w3id.org/smartenvironment/patterns/sensing.owl#Sensor"/>
            </owl:Restriction>
        </rdfs:subClassOf>
        <rdfs:comment xml:lang="en">Descibes a procedure required to configure a sensor to be used for an observation process in a smart environment context. This configuration can include both hardware ans software setup related to sensors such as the sampling rate, etc.</rdfs:comment>
        <rdfs:label xml:lang="en">configuration procedure</rdfs:label>
        <skos:example xml:lang="en">Descibes a procedure required to configure a sensor to be used for an observation process in a smart environment context. This configuration can include both hardware ans software setup related to sensors such as the sampling rate, etc.</skos:example>
    </owl:Class>
    


    <!-- https://w3id.org/smartenvironment/patterns/sensing.owl#Observation -->

    <owl:Class rdf:about="https://w3id.org/smartenvironment/patterns/sensing.owl#Observation">
        <rdfs:subClassOf rdf:resource="http://www.w3.org/ns/sosa/Observation"/>
        <rdfs:subClassOf>
            <owl:Restriction>
                <owl:onProperty rdf:resource="http://www.w3.org/ns/sosa/madeBySensor"/>
                <owl:someValuesFrom rdf:resource="https://w3id.org/smartenvironment/patterns/sensing.owl#Sensor"/>
            </owl:Restriction>
        </rdfs:subClassOf>
        <rdfs:comment xml:lang="en">Using a Sensor it describes the process of observing a property of a feature of interest.</rdfs:comment>
        <rdfs:label xml:lang="en">observation</rdfs:label>
        <skos:definition xml:lang="en">Using a Sensor it describes the process of observing a property of a feature of interest.</skos:definition>
    </owl:Class>
    


    <!-- https://w3id.org/smartenvironment/patterns/sensing.owl#Sensor -->

    <owl:Class rdf:about="https://w3id.org/smartenvironment/patterns/sensing.owl#Sensor">
        <rdfs:subClassOf rdf:resource="http://www.w3.org/ns/sosa/Sensor"/>
        <rdfs:subClassOf>
            <owl:Restriction>
                <owl:onProperty rdf:resource="http://www.w3.org/ns/sosa/madeObservation"/>
                <owl:someValuesFrom rdf:resource="https://w3id.org/smartenvironment/patterns/sensing.owl#Observation"/>
            </owl:Restriction>
        </rdfs:subClassOf>
        <rdfs:subClassOf>
            <owl:Restriction>
                <owl:onProperty rdf:resource="http://www.w3.org/ns/ssn/implements"/>
                <owl:someValuesFrom rdf:resource="https://w3id.org/smartenvironment/patterns/sensing.owl#ConfigurationProcedure"/>
            </owl:Restriction>
        </rdfs:subClassOf>
        <rdfs:comment xml:lang="en">Descibes a device that with a specific set of configuration is able to implements an observation process in order to monitor a property of a feature of interest in a smart environment.</rdfs:comment>
        <rdfs:label xml:lang="en">sensor</rdfs:label>
        <skos:definition xml:lang="en">Descibes a device that with a specific set of configuration is able to implements an observation process in order to monitor a property of a feature of interest in a smart environment.</skos:definition>
    </owl:Class>
</rdf:RDF>



<!-- Generated by the OWL API (version 4.2.6.20160910-2108) https://github.com/owlcs/owlapi -->

